ProofLibrary/Trigger.lean
@@ -6,36 +6,36 @@ structure PreTrigger where
   subs : GroundSubstitution
 
 namespace PreTrigger
-  def skolemize_var_or_const (trg : PreTrigger) (var_or_const : VarOrConst) : SkolemTerm :=
-    var_or_const.skolemize trg.rule.id trg.rule.frontier
+  def skolemize_var_or_const (trg : PreTrigger) (disjunctIndex : Nat) (var_or_const : VarOrConst) : SkolemTerm :=
+    var_or_const.skolemize trg.rule.id disjunctIndex trg.rule.frontier
 
   def apply_to_skolemized_term (trg : PreTrigger) (skolem_term : SkolemTerm) : GroundTerm :=
     trg.subs.apply_skolem_term skolem_term
 
-  def apply_to_var_or_const (trg : PreTrigger) : VarOrConst -> GroundTerm :=
-    (trg.apply_to_skolemized_term ∘ trg.skolemize_var_or_const)
+  def apply_to_var_or_const (trg : PreTrigger) (disjunctIndex : Nat) : VarOrConst -> GroundTerm :=
+    (trg.apply_to_skolemized_term ∘ (trg.skolemize_var_or_const disjunctIndex))
 
-  def apply_to_function_free_atom (trg : PreTrigger) (atom : FunctionFreeAtom) : Fact :=
+  def apply_to_function_free_atom (trg : PreTrigger) (disjunctIndex : Nat) (atom : FunctionFreeAtom) : Fact :=
     {
       predicate := atom.predicate
-      terms := atom.terms.map trg.apply_to_var_or_const
+      terms := atom.terms.map (trg.apply_to_var_or_const disjunctIndex)
     }
 
-  theorem apply_to_function_free_atom_terms_same_length (trg : PreTrigger) (atom : FunctionFreeAtom) : atom.terms.length = (trg.apply_to_function_free_atom atom).terms.length := by
+  theorem apply_to_function_free_atom_terms_same_length (trg : PreTrigger) (disjunctIndex : Nat) (atom : FunctionFreeAtom) : atom.terms.length = (trg.apply_to_function_free_atom disjunctIndex atom).terms.length := by
     unfold apply_to_function_free_atom
     simp
 
   def mapped_body (trg : PreTrigger) : List Fact := SubsTarget.apply trg.subs trg.rule.body
-  def mapped_head (trg : PreTrigger) : List (List Fact) := trg.rule.head.map (fun h => h.map trg.apply_to_function_free_atom)
+  def mapped_head (trg : PreTrigger) : List (List Fact) := trg.rule.head.enum.map (fun (i, h) => h.map (trg.apply_to_function_free_atom i))
 
   theorem head_length_eq_mapped_head_length (trg : PreTrigger) : trg.rule.head.length = trg.mapped_head.length := by
     unfold mapped_head
-    rw [List.length_map]
+    rw [List.length_map, List.length_enum]
 
   def result (trg : PreTrigger) : List FactSet :=
     trg.mapped_head.map List.toSet
 
-  theorem subs_application_is_injective_for_freshly_introduced_terms {t : Variable} (trg : PreTrigger) (t_not_in_frontier : ¬ t ∈ trg.rule.frontier) : ∀ s, (trg.apply_to_var_or_const (VarOrConst.var t) = trg.apply_to_var_or_const (VarOrConst.var s)) -> trg.skolemize_var_or_const (VarOrConst.var t) = trg.skolemize_var_or_const (VarOrConst.var s) := by
+  theorem subs_application_is_injective_for_freshly_introduced_terms {t : Variable} (trg : PreTrigger) (disjunctIndex : Fin trg.rule.head.length) (t_not_in_frontier : ¬ t ∈ trg.rule.frontier) : ∀ s, (trg.apply_to_var_or_const disjunctIndex (VarOrConst.var t) = trg.apply_to_var_or_const disjunctIndex (VarOrConst.var s)) -> trg.skolemize_var_or_const disjunctIndex (VarOrConst.var t) = trg.skolemize_var_or_const disjunctIndex (VarOrConst.var s) := by
     intro s apply_eq_for_t_and_s
 
     cases Decidable.em (s ∈ trg.rule.frontier) with
@@ -47,9 +47,9 @@ namespace PreTrigger
     | inl hl =>
       simp [t_not_in_frontier, hl, apply_to_var_or_const, apply_to_skolemized_term, skolemize_var_or_const, GroundSubstitution.apply_skolem_term, VarOrConst.skolemize] at apply_eq_for_t_and_s
       apply False.elim
-      let tree_for_s := trg.apply_to_var_or_const (VarOrConst.var s)
+      let tree_for_s := trg.apply_to_var_or_const disjunctIndex (VarOrConst.var s)
       let ts := trg.rule.frontier.map (fun fv => trg.subs fv)
-      let a : SkolemFS := { ruleId := trg.rule.id, var := t }
+      let a : SkolemFS := { ruleId := trg.rule.id, disjunctIndex, var := t }
       apply FiniteTree.tree_eq_while_contained_is_impossible tree_for_s (FiniteTreeList.fromList ts) a
       simp [tree_for_s, apply_to_var_or_const, apply_to_skolemized_term, skolemize_var_or_const, GroundSubstitution.apply_skolem_term, VarOrConst.skolemize, hl]
       apply apply_eq_for_t_and_s
@@ -64,12 +64,10 @@ namespace PreTrigger
     let disj_index_mapped_head : Fin trg.mapped_head.length := ⟨disj_index.val, (by have isLt := disj_index.isLt; unfold result at isLt; simp only [List.length_map] at isLt; exact isLt)⟩
     let fin_mapped := (trg.mapped_head.get disj_index_mapped_head).idx_of f ((trg.mapped_head.get disj_index_mapped_head).listToSetElementAlsoListElement f (by unfold result at f_in_res; simp at f_in_res; apply f_in_res))
     have fin_mapped_isLt := fin_mapped.isLt
-    ⟨fin_mapped.val, by simp [mapped_head, List.length_map] at fin_mapped_isLt; exact fin_mapped_isLt⟩
+    ⟨fin_mapped.val, by simp [mapped_head] at fin_mapped_isLt; exact fin_mapped_isLt⟩
 
-  theorem apply_subs_to_atom_at_idx_same_as_fact_at_idx (trg : PreTrigger) (disj_index : Fin trg.rule.head.length) (idx : Fin (trg.rule.head.get disj_index).length) : trg.apply_to_function_free_atom ((trg.rule.head.get disj_index).get idx) = (trg.mapped_head.get ⟨disj_index.val, (by rw [← head_length_eq_mapped_head_length]; exact disj_index.isLt)⟩).get ⟨idx.val, (by unfold mapped_head; simp)⟩ := by
+  theorem apply_subs_to_atom_at_idx_same_as_fact_at_idx (trg : PreTrigger) (disj_index : Fin trg.rule.head.length) (idx : Fin (trg.rule.head.get disj_index).length) : trg.apply_to_function_free_atom disj_index ((trg.rule.head.get disj_index).get idx) = (trg.mapped_head.get ⟨disj_index.val, (by rw [← head_length_eq_mapped_head_length]; exact disj_index.isLt)⟩).get ⟨idx.val, (by unfold mapped_head; simp)⟩ := by
     unfold mapped_head
-    have : (trg.rule.head.map (fun h => h.map trg.apply_to_function_free_atom)).get ⟨disj_index.val, (by rw [List.length_map]; exact disj_index.isLt)⟩ = (trg.rule.head.get disj_index).map trg.apply_to_function_free_atom := by simp
-    rw [List.get_eq_of_eq this]
     simp
 
   def loaded (trg : PreTrigger) (F : FactSet) : Prop :=
@@ -108,6 +106,48 @@ namespace PreTrigger
         apply ih
         intro _ hf'; apply base; apply Or.inr; apply hf'
         exact hr
+
+  def equiv (trg1 trg2 : PreTrigger) : Prop := trg1.rule = trg2.rule ∧ ∀ v, v ∈ trg1.rule.frontier.toSet -> trg1.subs v = trg2.subs v
+
+  theorem result_eq_of_equiv (trg1 trg2 : PreTrigger) : trg1.equiv trg2 -> trg1.result = trg2.result := by
+    unfold equiv
+    intro h
+
+    /- unfold result -/
+    /- simp -/
+
+    have : trg1.mapped_head = trg2.mapped_head := by
+      unfold mapped_head
+      rw [h.left]
+      rw [List.map_eq_map_iff]
+      intro _ _
+      unfold PreTrigger.apply_to_function_free_atom
+      simp
+      intro a _ voc hvoc
+      cases voc with
+      | const c => simp [PreTrigger.apply_to_var_or_const, PreTrigger.apply_to_skolemized_term, PreTrigger.skolemize_var_or_const, GroundSubstitution.apply_skolem_term, VarOrConst.skolemize]
+      | var v =>
+        cases Decidable.em (v ∈ trg1.rule.frontier) with
+        | inl v_in_frontier =>
+          simp [PreTrigger.apply_to_var_or_const, PreTrigger.apply_to_skolemized_term, PreTrigger.skolemize_var_or_const, GroundSubstitution.apply_skolem_term]
+          rw [← h.left]
+          simp [VarOrConst.skolemize, v_in_frontier]
+          apply h.right
+          apply List.listElementAlsoToSetElement
+          apply v_in_frontier
+        | inr v_not_in_frontier =>
+          simp [PreTrigger.apply_to_var_or_const, PreTrigger.apply_to_skolemized_term, PreTrigger.skolemize_var_or_const, GroundSubstitution.apply_skolem_term]
+          rw [← h.left]
+          simp [VarOrConst.skolemize, v_not_in_frontier]
+          apply congrArg
+          rw [← FiniteTreeList.eqIffFromListEq]
+          apply List.map_eq_map_if_functions_eq
+          intro w hw
+          rw [← h.right w]
+          exact hw
+
+    unfold result
+    rw [this]
 end PreTrigger
 
 structure ObsoletenessCondition where
@@ -144,17 +184,22 @@ def SkolemObsoleteness : ObsoletenessCondition := {
     intro trg F
     simp
     intro i h
-    exists (fun v => trg.apply_to_var_or_const (VarOrConst.var v))
+    exists (fun v => trg.apply_to_var_or_const i (VarOrConst.var v))
     constructor
     . intro v v_in_frontier
       simp [PreTrigger.apply_to_var_or_const, PreTrigger.apply_to_skolemized_term, GroundSubstitution.apply_skolem_term, PreTrigger.skolemize_var_or_const, VarOrConst.skolemize, v_in_frontier]
     . exists ⟨i, by rw [PreTrigger.head_length_eq_mapped_head_length]; exact i.isLt⟩
-      unfold PreTrigger.mapped_head at h
+      have : trg.mapped_head[i.val] = (trg.rule.head[i]'(by rw [PreTrigger.head_length_eq_mapped_head_length]; exact i.isLt)).map (fun a => { predicate := a.predicate, terms := a.terms.map (trg.apply_to_var_or_const i)}) := by
+        unfold PreTrigger.mapped_head
+        unfold PreTrigger.apply_to_function_free_atom
+        simp
+        rfl
+      rw [this] at h
+
       unfold GroundSubstitution.apply_function_free_conj
-      unfold PreTrigger.apply_to_function_free_atom at h
       unfold GroundSubstitution.apply_function_free_atom
-      simp at h
-      have : GroundSubstitution.apply_var_or_const (fun v => trg.apply_to_var_or_const (VarOrConst.var v)) = trg.apply_to_var_or_const := by
+
+      have : GroundSubstitution.apply_var_or_const (fun v => trg.apply_to_var_or_const i (VarOrConst.var v)) = trg.apply_to_var_or_const i := by
         unfold GroundSubstitution.apply_var_or_const
         apply funext
         intro x
@@ -162,6 +207,7 @@ def SkolemObsoleteness : ObsoletenessCondition := {
         | var => rfl
         | const => simp [PreTrigger.apply_to_var_or_const, PreTrigger.apply_to_skolemized_term, GroundSubstitution.apply_skolem_term, PreTrigger.skolemize_var_or_const, VarOrConst.skolemize]
       rw [this]
+
       apply h
   contains_trg_result_implies_cond := by
     intro trg F i result_in_F
@@ -192,10 +238,11 @@ def RestrictedObsoleteness : ObsoletenessCondition := {
   cond_implies_trg_is_satisfied := by intro _ _ h; exact h
   contains_trg_result_implies_cond := by
     intro trg F i result_in_F
-    let obs_subs := fun v : Variable => trg.apply_to_var_or_const (VarOrConst.var v)
+    let adjusted_i : Fin trg.rule.head.length := ⟨i, by rw [PreTrigger.head_length_eq_mapped_head_length]; have isLt := i.isLt; unfold PreTrigger.result at isLt; simp [List.length_map] at isLt; exact isLt⟩
+    let obs_subs := fun v : Variable => trg.apply_to_var_or_const adjusted_i (VarOrConst.var v)
 
     exists obs_subs
-    exists ⟨i, by rw [PreTrigger.head_length_eq_mapped_head_length]; have isLt := i.isLt; unfold PreTrigger.result at isLt; simp [List.length_map] at isLt; exact isLt⟩
+    exists adjusted_i
     constructor
     . intro _ v'_in_frontier
       simp [obs_subs, PreTrigger.apply_to_var_or_const, PreTrigger.apply_to_skolemized_term, PreTrigger.skolemize_var_or_const, GroundSubstitution.apply_skolem_term, VarOrConst.skolemize, v'_in_frontier]
@@ -207,7 +254,7 @@ def RestrictedObsoleteness : ObsoletenessCondition := {
       unfold PreTrigger.mapped_head
       unfold PreTrigger.apply_to_function_free_atom
 
-      have : ∀ a : FunctionFreeAtom, (List.map (GroundSubstitution.apply_var_or_const obs_subs) a.terms) = (List.map (trg.apply_to_var_or_const) a.terms) := by
+      have : ∀ a : FunctionFreeAtom, (List.map (GroundSubstitution.apply_var_or_const obs_subs) a.terms) = (List.map (trg.apply_to_var_or_const adjusted_i) a.terms) := by
         intro a
         induction a.terms with
         | nil => simp [List.map]
@@ -218,6 +265,8 @@ def RestrictedObsoleteness : ObsoletenessCondition := {
           | var v => simp
           | const c => simp [VarOrConst.skolemize]
 
+      simp
+      simp only [adjusted_i] at this
       simp [← this]
       apply hf'
 }
@@ -248,16 +297,20 @@ end FactSet
 def RTrigger (obs : ObsoletenessCondition)(r : RuleSet) := { trg : Trigger obs // trg.rule ∈ r.rules}
 
 namespace RTrigger
+  def equiv (trg1 trg2 : RTrigger obs rs) : Prop := trg1.val.equiv trg2.val
+
   theorem funcTermForExisVarInMultipleTriggersMeansTheyAreTheSame
     {rs : RuleSet}
     (trg1 trg2 : RTrigger obs rs)
+    (disjIndex1 : Fin trg1.val.rule.head.length)
+    (disjIndex2 : Fin trg2.val.rule.head.length)
     (var1 var2 : Variable)
     (var1_not_in_frontier : ¬ var1 ∈ trg1.val.rule.frontier)
     (var2_not_in_frontier : ¬ var2 ∈ trg2.val.rule.frontier)
     :
-    (trg1.val.apply_to_var_or_const (VarOrConst.var var1)) = (trg2.val.apply_to_var_or_const (VarOrConst.var var2))
+    (trg1.val.apply_to_var_or_const disjIndex1 (VarOrConst.var var1)) = (trg2.val.apply_to_var_or_const disjIndex2 (VarOrConst.var var2))
     ->
-    trg1.val.rule = trg2.val.rule ∧ ∀ v, v ∈ trg1.val.rule.frontier.toSet -> trg1.val.subs v = trg2.val.subs v := by
+    trg1.equiv trg2 ∧ disjIndex1.val = disjIndex2.val := by
     intro applications_eq
     simp [PreTrigger.apply_to_var_or_const, PreTrigger.apply_to_skolemized_term, PreTrigger.skolemize_var_or_const, GroundSubstitution.apply_skolem_term, VarOrConst.skolemize, var1_not_in_frontier, var2_not_in_frontier] at applications_eq
     injection applications_eq with rule_ids_and_vars_eq arguments_eq
@@ -270,13 +323,18 @@ namespace RTrigger
       exact trg2.property
       exact rule_ids_and_vars_eq.left
     constructor
-    . exact rules_eq
-    . let right := arguments_eq
-      rw [← FiniteTreeList.eqIffFromListEq _ _] at right
-      have : trg1.val.rule.frontier = trg2.val.rule.frontier := by rw [rules_eq]
-      rw [← this] at right
-      rw [List.map_eq_map_iff] at right
-      intro v
-      rw [← List.inIffInToSet]
-      apply right
+    . unfold equiv
+      unfold PreTrigger.equiv
+      constructor
+      . exact rules_eq
+      . let right := arguments_eq
+        rw [← FiniteTreeList.eqIffFromListEq _ _] at right
+        have : trg1.val.rule.frontier = trg2.val.rule.frontier := by rw [rules_eq]
+        rw [← this] at right
+        rw [List.map_eq_map_iff] at right
+        intro v
+        rw [← List.inIffInToSet]
+        apply right
+    . exact rule_ids_and_vars_eq.right.left
 end RTrigger
+
