ProofLibrary/PossiblyInfiniteTree.lean
@@ -10,14 +10,14 @@ def InfiniteTreeSkeleton (α : Type u) := (List Nat) -> α
 namespace InfiniteTreeSkeleton
   def children (tree : InfiniteTreeSkeleton α) (node : List Nat) : InfiniteList α := fun n => tree (n :: node)
 
-  def branches (tree : InfiniteTreeSkeleton α) : Set (InfiniteList α) := fun branch => 
-    ∃ nodes : InfiniteList Nat, ∀ n : Nat, branch n = tree (nodes.take n).reverse 
+  def branches (tree : InfiniteTreeSkeleton α) : Set (InfiniteList α) := fun branch =>
+    ∃ nodes : InfiniteList Nat, ∀ n : Nat, branch n = tree (nodes.take n).reverse
 
-  def branches_through (tree : InfiniteTreeSkeleton α) (node : List Nat) : Set (InfiniteList α) := fun branch => 
+  def branches_through (tree : InfiniteTreeSkeleton α) (node : List Nat) : Set (InfiniteList α) := fun branch =>
     branch ∈ tree.branches ∧ ∀ (i : Fin (node.length + 1)), branch i = tree (node.drop (node.length-i))
 end InfiniteTreeSkeleton
 
-structure PossiblyInfiniteTree (α : Type u) where 
+structure PossiblyInfiniteTree (α : Type u) where
   infinite_tree : InfiniteTreeSkeleton (Option α)
   no_orphans : ∀ node : List Nat, infinite_tree node ≠ none -> ∀ parent : { l : List Nat // ∃ diff, diff ++ l = node }, infinite_tree parent ≠ none
   no_holes_in_children : ∀ node : List Nat, ∀ n : Nat, (infinite_tree.children node) n ≠ none -> ∀ m : Fin n, (infinite_tree.children node) m ≠ none
@@ -30,7 +30,7 @@ namespace PossiblyInfiniteTree
     no_holes := by apply tree.no_holes_in_children
   }
 
-  theorem children_empty_when_not_existing (tree : PossiblyInfiniteTree α) (node : List Nat) : tree.get node = none -> tree.children node = PossiblyInfiniteList.empty := by 
+  theorem children_empty_when_not_existing (tree : PossiblyInfiniteTree α) (node : List Nat) : tree.get node = none -> tree.children node = PossiblyInfiniteList.empty := by
     intro h
     unfold children
     unfold PossiblyInfiniteList.empty
@@ -41,13 +41,13 @@ namespace PossiblyInfiniteTree
     apply dec.byContradiction
     intro contra
     let parent : { l : List Nat // ∃ diff, diff ++ l = index :: node } := ⟨node, by exists [index]⟩
-    have : tree.infinite_tree parent ≠ none := by 
+    have : tree.infinite_tree parent ≠ none := by
       apply no_orphans
       unfold InfiniteTreeSkeleton.children at contra
       exact contra
     contradiction
 
-  theorem children_empty_means_all_following_none (tree : PossiblyInfiniteTree α) (node : List Nat) : tree.children node = PossiblyInfiniteList.empty -> ∀ i, tree.get (i :: node) = none := by 
+  theorem children_empty_means_all_following_none (tree : PossiblyInfiniteTree α) (node : List Nat) : tree.children node = PossiblyInfiniteList.empty -> ∀ i, tree.get (i :: node) = none := by
     intro h i
     unfold get
     unfold children at h
@@ -57,49 +57,74 @@ namespace PossiblyInfiniteTree
     apply congr h
     rfl
 
-  def branches (tree : PossiblyInfiniteTree α) : Set (PossiblyInfiniteList α) := fun pil => 
+  theorem first_child_none_means_children_empty (tree : PossiblyInfiniteTree α) (node : List Nat) : tree.get (0::node) = none -> tree.children node = PossiblyInfiniteList.empty := by
+    intro h
+    unfold PossiblyInfiniteList.empty
+    unfold children
+    unfold InfiniteTreeSkeleton.children
+    simp
+    apply funext
+    intro n
+    cases n with
+    | zero => exact h
+    | succ n =>
+      apply Option.decidable_eq_none.byContradiction
+      intro contra
+      have no_holes := tree.no_holes_in_children node (n+1)
+      unfold children at no_holes
+      unfold InfiniteTreeSkeleton.children at no_holes
+      specialize no_holes contra ⟨0, by simp⟩
+      contradiction
+
+  theorem getElem_children_eq_get_tree (tree : PossiblyInfiniteTree α) (node : List Nat) (index : Nat) : (tree.children node).infinite_list index = tree.get (index :: node) := by
+    unfold children
+    unfold get
+    unfold InfiniteTreeSkeleton.children
+    simp
+
+  def branches (tree : PossiblyInfiniteTree α) : Set (PossiblyInfiniteList α) := fun pil =>
     pil.infinite_list ∈ tree.infinite_tree.branches
 
-  def branches_through (tree : PossiblyInfiniteTree α) (node : List Nat) : Set (PossiblyInfiniteList α) := fun pil => 
+  def branches_through (tree : PossiblyInfiniteTree α) (node : List Nat) : Set (PossiblyInfiniteList α) := fun pil =>
     pil.infinite_list ∈ tree.infinite_tree.branches_through node
 
   def leaves (tree : PossiblyInfiniteTree α) : Set α := fun a => ∃ node : List Nat, tree.get node = some a ∧ tree.children node = PossiblyInfiniteList.empty
 end PossiblyInfiniteTree
 
-structure FiniteDegreeTree (α : Type u) where 
-  tree : PossiblyInfiniteTree α 
+structure FiniteDegreeTree (α : Type u) where
+  tree : PossiblyInfiniteTree α
   finitely_many_children : ∀ node : List Nat, ∃ k, (tree.children node).infinite_list k = none ∧ ∀ k' : Fin k, (tree.children node).infinite_list k' ≠ none
 
 namespace FiniteDegreeTree
   def get (tree : FiniteDegreeTree α) (node : List Nat) : Option α := tree.tree.get node
 
-  def children (tree : FiniteDegreeTree α) (node : List Nat) : List α := 
-    let rec loop (n : Nat) : List α := match eq : (tree.tree.children node).infinite_list n with 
+  def children (tree : FiniteDegreeTree α) (node : List Nat) : List α :=
+    let rec loop (n : Nat) : List α := match eq : (tree.tree.children node).infinite_list n with
       | .none => []
-      | .some a => 
-        have : Classical.choose (tree.finitely_many_children node) - (n+1) < Classical.choose (tree.finitely_many_children node) - n := by 
+      | .some a =>
+        have : Classical.choose (tree.finitely_many_children node) - (n+1) < Classical.choose (tree.finitely_many_children node) - n := by
           apply Nat.sub_add_lt_sub
           . apply Classical.byContradiction
-            intro contra 
+            intro contra
             simp at contra
             have hk_none := (Classical.choose_spec (tree.finitely_many_children node)).left
-            have hk_not_none : (tree.tree.children node).infinite_list (Classical.choose (tree.finitely_many_children node)) ≠ none := by 
+            have hk_not_none : (tree.tree.children node).infinite_list (Classical.choose (tree.finitely_many_children node)) ≠ none := by
               simp only [PossiblyInfiniteTree.children]
               simp only [PossiblyInfiniteTree.children] at eq
-              have goal := 
-                tree.tree.no_holes_in_children 
-                node 
-                n 
-                (by apply Option.someNotNone; apply eq) 
-                ⟨Classical.choose (tree.finitely_many_children node), by 
-                  cases Nat.eq_or_lt_of_le (Nat.le_of_lt_succ contra) with 
-                  | inl hl => 
+              have goal :=
+                tree.tree.no_holes_in_children
+                node
+                n
+                (by apply Option.someNotNone; apply eq)
+                ⟨Classical.choose (tree.finitely_many_children node), by
+                  cases Nat.eq_or_lt_of_le (Nat.le_of_lt_succ contra) with
+                  | inl hl =>
                     simp only [PossiblyInfiniteTree.children] at hk_none
                     rw [hl] at hk_none
                     have eq_not_none := Option.someNotNone eq
                     contradiction
                   | inr hr => exact hr
-                ⟩ 
+                ⟩
               exact goal
             contradiction
           . simp
@@ -107,11 +132,11 @@ namespace FiniteDegreeTree
     termination_by Classical.choose (tree.finitely_many_children node) - n
     loop 0
 
-    theorem in_children_loop_iff_step (tree : FiniteDegreeTree α) (node : List Nat) : ∀ (el : α) (n : Nat), (el ∈ children.loop tree node n) ↔ ((some el = (tree.tree.children node).infinite_list n) ∨ el ∈ children.loop tree node (n+1)) := by 
+    theorem in_children_loop_iff_step (tree : FiniteDegreeTree α) (node : List Nat) : ∀ (el : α) (n : Nat), (el ∈ children.loop tree node n) ↔ ((some el = (tree.tree.children node).infinite_list n) ∨ el ∈ children.loop tree node (n+1)) := by
     intro el n
-    cases eq : (tree.tree.children node).infinite_list n with 
-    | none => 
-      simp 
+    cases eq : (tree.tree.children node).infinite_list n with
+    | none =>
+      simp
       unfold children.loop
       constructor
       . intro contra
@@ -119,106 +144,106 @@ namespace FiniteDegreeTree
         simp [eq] at contra
         split at contra
         . contradiction
-        case h_2 _ heq => 
+        case h_2 _ heq =>
           rw [eq] at heq
           contradiction
       . intro h
         let fin : Fin (n+1) := ⟨n, by simp⟩
-        have : ¬ (tree.tree.children node).infinite_list fin = none := by 
+        have : ¬ (tree.tree.children node).infinite_list fin = none := by
           apply tree.tree.no_holes_in_children
-          cases eq2 : (tree.tree.children node).infinite_list (n+1) with 
-          | none => 
+          cases eq2 : (tree.tree.children node).infinite_list (n+1) with
+          | none =>
             split at h
             . contradiction
-            case a.none.h_2 _ heq => 
+            case a.none.h_2 _ heq =>
               rw [eq2] at heq
               contradiction
-          | some a => 
-            apply Option.someNotNone 
+          | some a =>
+            apply Option.someNotNone
             apply eq2
         contradiction
-    | some a => 
+    | some a =>
       constructor
       . intro h
         unfold children.loop at h
         split at h
         . contradiction
-        case h_2 a' heq => 
+        case h_2 a' heq =>
           simp at h
-          cases h with 
+          cases h with
           | inl h => apply Or.inl; rw [h, ←eq, heq]
           | inr h => apply Or.inr; apply h
       . intro h
         unfold children.loop
         split
         case h_1 heq => rw [heq] at eq; contradiction
-        case h_2 a heq => 
+        case h_2 a heq =>
           simp
-          cases h with 
+          cases h with
           | inl h => apply Or.inl; rw [heq] at eq; injection eq with eq; injection h with h; rw [h, eq]
           | inr h => apply Or.inr; apply h
 
-  theorem in_children_loop_iff (tree : FiniteDegreeTree α) (node : List Nat) : ∀ (el : α) (n m : Nat), (el ∈ children.loop tree node n) ↔ ((∃ i : Fin m, some el = (tree.tree.children node).infinite_list (n+i)) ∨ el ∈ children.loop tree node (n+m)) := by 
+  theorem in_children_loop_iff (tree : FiniteDegreeTree α) (node : List Nat) : ∀ (el : α) (n m : Nat), (el ∈ children.loop tree node n) ↔ ((∃ i : Fin m, some el = (tree.tree.children node).infinite_list (n+i)) ∨ el ∈ children.loop tree node (n+m)) := by
     intro el n m
-    
-    induction m with 
+
+    induction m with
     | zero => simp; intro i; have contra := i.isLt; contradiction
     | succ m ih =>
       rw [ih]
       constructor
       . intro h
-        cases h with 
-        | inl h => 
+        cases h with
+        | inl h =>
           apply Or.inl
-          cases h with | intro i hi => 
-            exists ⟨i.val, by apply Nat.lt_trans; apply i.isLt; simp⟩  
-        | inr h => 
+          cases h with | intro i hi =>
+            exists ⟨i.val, by apply Nat.lt_trans; apply i.isLt; simp⟩
+        | inr h =>
           have h_iff_step := (tree.in_children_loop_iff_step node el (n + m)).mp h
-          cases h_iff_step with 
-          | inl h => 
+          cases h_iff_step with
+          | inl h =>
             apply Or.inl
-            let fin : Fin (m+1) := ⟨m, by simp⟩ 
+            let fin : Fin (m+1) := ⟨m, by simp⟩
             exists fin
           | inr h => apply Or.inr; apply h
       . intro h
-        cases h with 
-        | inl h => 
+        cases h with
+        | inl h =>
           rw [tree.in_children_loop_iff_step]
           rw [← or_assoc]
           apply Or.inl
           cases h with | intro i hi =>
             have fin_cases := i.eq_last_or_prev_fin
-            cases fin_cases with 
+            cases fin_cases with
             | inl h => rw [h] at hi; apply Or.inr; apply hi
-            | inr h => 
-              cases h with | intro j hj => 
+            | inr h =>
+              cases h with | intro j hj =>
                 rw [hj] at hi
                 apply Or.inl
                 exists j
-        | inr h => 
+        | inr h =>
           apply Or.inr
           rw [tree.in_children_loop_iff_step]
-          apply Or.inr 
+          apply Or.inr
           apply h
 
-  theorem in_children_iff_loop_index_exists (tree : FiniteDegreeTree α) (node : List Nat) : ∀ (el : α), (el ∈ tree.children node) ↔ (∃ n l, (children.loop tree node n) = el :: l) := by 
+  theorem in_children_iff_loop_index_exists (tree : FiniteDegreeTree α) (node : List Nat) : ∀ (el : α), (el ∈ tree.children node) ↔ (∃ n l, (children.loop tree node n) = el :: l) := by
     intro el
     unfold children
     constructor
     . cases tree.finitely_many_children node with | intro k hk =>
         rw [tree.in_children_loop_iff node el 0 k]
         intro h
-        cases h with 
-        | inr h => 
+        cases h with
+        | inr h =>
           simp at h
           unfold children.loop at h
           split at h
           . contradiction
-          case h_2 a heq => 
+          case h_2 a heq =>
             have contra := hk.left
             rw [heq] at contra
             contradiction
-        | inl h => 
+        | inl h =>
           cases h with | intro i hi =>
             simp at hi
             exists i
@@ -226,7 +251,7 @@ namespace FiniteDegreeTree
             conv => left; unfold children.loop
             split
             case h_1 heq => rw [heq] at hi; contradiction
-            case h_2 a heq => 
+            case h_2 a heq =>
               simp
               rw [heq] at hi
               injection hi with hi
@@ -239,17 +264,17 @@ namespace FiniteDegreeTree
         rw [h]
         simp
 
-  theorem in_children_iff_index_exists (tree : FiniteDegreeTree α) (node : List Nat) : ∀ (el : α), (el ∈ tree.children node) ↔ (∃ n, (tree.tree.children node).infinite_list n = some el) := by 
+  theorem in_children_iff_index_exists (tree : FiniteDegreeTree α) (node : List Nat) : ∀ (el : α), (el ∈ tree.children node) ↔ (∃ n, (tree.tree.children node).infinite_list n = some el) := by
     intro el
     rw [in_children_iff_loop_index_exists]
-    constructor 
-    . intro h 
+    constructor
+    . intro h
       cases h with | intro n h => cases h with | intro l h =>
         exists n
         unfold children.loop at h
         split at h
         . contradiction
-        case h_2 a heq => 
+        case h_2 a heq =>
           simp at h
           rw [heq]
           rw [h.left]
@@ -260,12 +285,12 @@ namespace FiniteDegreeTree
         conv => left; unfold children.loop
         split
         case h_1 heq => rw [heq] at h; contradiction
-        case h_2 a heq => 
+        case h_2 a heq =>
           simp
           rw [heq] at h
           injection h
 
-  theorem children_empty_when_not_existing (tree : FiniteDegreeTree α) (node : List Nat) : tree.get node = none -> tree.children node = [] := by 
+  theorem children_empty_when_not_existing (tree : FiniteDegreeTree α) (node : List Nat) : tree.get node = none -> tree.children node = [] := by
     intro h
     unfold children
     unfold children.loop
@@ -275,14 +300,14 @@ namespace FiniteDegreeTree
     simp
     rw [this]
 
-  theorem children_empty_means_all_following_none (tree : FiniteDegreeTree α) (node : List Nat) : tree.children node = [] -> ∀ i, tree.get (i :: node) = none := by 
-    intro h 
+  theorem children_empty_means_all_following_none (tree : FiniteDegreeTree α) (node : List Nat) : tree.children node = [] -> ∀ i, tree.get (i :: node) = none := by
+    intro h
     unfold children at h
     unfold children.loop at h
     unfold get
     apply PossiblyInfiniteTree.children_empty_means_all_following_none
 
-    have zero_th_child_none : (tree.tree.children node).infinite_list 0 = none := by 
+    have zero_th_child_none : (tree.tree.children node).infinite_list 0 = none := by
       have dec : Decidable ((tree.tree.children node).infinite_list 0 = none) := Option.decidable_eq_none
       apply dec.byContradiction
       intro contra
@@ -290,16 +315,16 @@ namespace FiniteDegreeTree
       . contradiction
       . simp at h
 
-    have : ∀ i, (tree.tree.children node).infinite_list i = none := by 
+    have : ∀ i, (tree.tree.children node).infinite_list i = none := by
       intro i
-      cases i with 
+      cases i with
       | zero => apply zero_th_child_none
-      | succ i => 
+      | succ i =>
         have dec : Decidable ((tree.tree.children node).infinite_list (i+1) = none) := Option.decidable_eq_none
         apply dec.byContradiction
         intro contra
         let zero_fin : Fin (i+1) := ⟨0, by simp⟩
-        have : ¬ (tree.tree.children node).infinite_list zero_fin = none := by 
+        have : ¬ (tree.tree.children node).infinite_list zero_fin = none := by
           apply (tree.tree.children node).no_holes
           apply contra
         contradiction
@@ -310,6 +335,54 @@ namespace FiniteDegreeTree
     unfold PossiblyInfiniteTree.children at this
     simp at this
     apply this
+
+  theorem first_child_none_means_children_empty (tree : FiniteDegreeTree α) (node : List Nat) : tree.get (0::node) = none -> tree.children node = [] := by
+    intro h
+    have lifted_children_none := tree.tree.first_child_none_means_children_empty node h
+    unfold children
+    unfold children.loop
+    split
+    case h_1 _ => rfl
+    case h_2 heq => rw [lifted_children_none] at heq; simp [PossiblyInfiniteList.empty] at heq
+
+  theorem getElem_children_eq_loop_at_index (tree : FiniteDegreeTree α) (node : List Nat) (index : Nat) : ∀ c, (children.loop tree node c)[index]? = (children.loop tree node (index + c))[0]? := by
+    induction index with
+    | zero => simp
+    | succ index ih =>
+      intro c
+      conv => left; unfold children.loop
+      split
+      case h_1 heq =>
+        unfold children.loop
+        have : (tree.tree.children node).infinite_list (index + 1 + c) = none := by
+          apply Option.decidable_eq_none.byContradiction
+          intro contra
+          let m : Fin (index + 1 + c) := ⟨c, by simp⟩
+          apply (tree.tree.children node).no_holes (index + 1 + c) contra m
+          simp [m]
+          exact heq
+        simp
+        rw [this]
+        simp
+      case h_2 heq =>
+        simp
+        rw [ih]
+        rw [Nat.add_assoc, Nat.add_comm c 1]
+
+  theorem getElem_children_eq_getElem_tree_children (tree : FiniteDegreeTree α) (node : List Nat) (index : Nat) : (tree.children node)[index]? = (tree.tree.children node).infinite_list index := by
+    unfold children
+    rw [getElem_children_eq_loop_at_index]
+    simp
+    unfold children.loop
+    split
+    case h_1 heq => rw [heq]; simp
+    case h_2 heq => simp; rw [heq]
+
+  theorem getElem_children_eq_get_tree (tree : FiniteDegreeTree α) (node : List Nat) (index : Fin (tree.children node).length) : (tree.children node)[index.val] = tree.get (index.val :: node) := by
+    unfold get
+    rw [← List.getElem?_eq_getElem]
+    rw [getElem_children_eq_getElem_tree_children]
+    apply PossiblyInfiniteTree.getElem_children_eq_get_tree
 
   def branches (tree : FiniteDegreeTree α) : Set (PossiblyInfiniteList α) := tree.tree.branches
 
